\subsection*{Aufgabe 9 - HML mit Rekursion}

\subsubsection*{a)}

Die zugrunde liegende Formel ist
$ X \HMmin ( \poss {a} \true \lor \poss{c} \true ) \land \necess {Act} X $. \\

\begin{align*}
\OSem{ (\poss{a} \true \lor \poss{c} \true ) \land \necess{Act} X }{\emptyset}
=& ( \possDenot{a} \Proc \cup \possDenot{c}\Proc) \cap
 (\necessDenot{a}\emptyset \cap \necessDenot{b} \emptyset \cap \necessDenot{c} \emptyset)\\
=& (\{ p_1, p_2, p_6, p_7, p_8 \} \cup \{p_4, p_6, p_7\}) \cap\\
  &( \{p_3, p_4, p_5, p_9 \} \cap
  \{p_1, p_3, p_5, p_7, p_8, p_9 \} \cap
  \{p_1, p_2, p_3, p_5, p_8, p_9 \}) \\
=& \{p_1, p_2, p_4, p_6, p_7, p_8 \} \cap \{ p_3, p_5, p_9 \} \\
=& \emptyset
\end{align*}

An dieser Stelle haben wir einen Fixpunkt erreicht, da
$ \OSem {(\poss {a} \true \lor \poss{c} \true ) \land \necess {Act} X }{\emptyset} = \emptyset $.


\subsubsection*{b)}

Die zugrunde liegende Formel ist
$ X \HMmax ( \poss {a} \true \lor \poss{c} \true ) \land \poss{Act} X $. \\

% O^1
\begin{align*}
\OSem{ (\poss{a} \true \lor \poss{c} \true ) \land \poss{Act} X }{\Proc}
=& ( \possDenot{a} \Proc \cup \possDenot{c}\Proc) \cap
 (\possDenot{a}\Proc \cap \possDenot{b} \Proc \cap \possDenot{c} \Proc)\\
=& (\{ p_1, p_2, p_6, p_7, p_8 \} \cup \{p_4, p_6, p_7\}) \cap\\
  &(\{ p_1, p_2, p_6, p_7, p_8 \} \cup
   \{p_2, p_4, p_6\}) \cup
   \{p_4, p_6, p_7\}) \cup\\
=& \{p_1, p_2, p_4, p_6, p_7, p_8 \} \cap \Proc \setminus \{ p_3, p_5, p_9 \} \\
=& \{p_1, p_2, p_4, p_6, p_7, p_8 \}
\end{align*}

% O^2
\begin{align*}
(\OSem{ (\poss{a} \true \lor \poss{c} \true ) \land \poss{Act} X }{})^2 (\Proc)
=& \OSem{ (\poss{a} \true \lor \poss{c} \true ) \land \poss{Act} X }
   { \{p_1, p_2, p_4, p_6, p_7, p_8 \}} \\
=& ( \possDenot{a} \Proc \cup \possDenot{c}\Proc) \cap \\
  &(\possDenot{a} \{p_1, p_2, p_4, p_6, p_7, p_8 \} \cup \\
  &\possDenot{b} \{p_1, p_2, p_4, p_6, p_7, p_8 \}  \cup \\
  &\possDenot{c}  \{p_1, p_2, p_4, p_6, p_7, p_8 \})\\
=& (\{ p_1, p_2, p_6, p_7, p_8 \} \cup \{p_4, p_6, p_7\}) \cap\\
   &(\{ p_6, p_8 \} \cup
   \{p_2, p_6\} \cup
   \{p_4, p_7\})\\
=& \{p_1, p_2, p_4, p_6, p_7, p_8 \} \cap  \{ p_2, p_4, p_6, p_7, p_8 \} \\
=& \{p_2, p_4, p_6, p_7, p_8 \}
\end{align*}

% O^3
\begin{align*}
(\OSem{ (\poss{a} \true \lor \poss{c} \true ) \land \poss{Act} X }{})^3 (\Proc)
=& \OSem{ (\poss{a} \true \lor \poss{c} \true ) \land \poss{Act} X }
   { \{p_2, p_4, p_6, p_7, p_8 \}} \\
=& ( \possDenot{a} \Proc \cup \possDenot{c}\Proc) \cap \\
  &(\possDenot{a} \{p_2, p_4, p_6, p_7, p_8 \} \cap \\
  &\possDenot{b} \{ p_2, p_4, p_6, p_7, p_8 \}  \cap \\
  &\possDenot{c}  \{p_2, p_4, p_6, p_7, p_8 \})\\
=& (\{ p_1, p_2, p_6, p_7, p_8 \} \cup \{p_4, p_6, p_7\}) \cap\\
   &(\{ p_6, p_8 \} \cup
   \{p_6\} \cup
   \{p_4, p_7\}) \\
=& \{p_1, p_2, p_4, p_6, p_7, p_8 \} \cap  \{ p_4, p_6, p_7, p_8 \} \\
=& \{p_4, p_6, p_7, p_8 \}
\end{align*}

% O^4
\begin{align*}
(\OSem{ (\poss{a} \true \lor \poss{c} \true ) \land \poss{Act} X }{})^4 (\Proc)
=& \OSem{ (\poss{a} \true \lor \poss{c} \true ) \land \poss{Act} X }
   { \{p_4, p_6, p_7, p_8 \}} \\
=& ( \possDenot{a} \Proc \cup \possDenot{c}\Proc) \cap \\
  &(\possDenot{a} \{p_4, p_6, p_7, p_8 \} \cap
  \possDenot{b} \{ p_4, p_6, p_7, p_8 \}  \cap
  \possDenot{c}  \{ p_4, p_6, p_7, p_8 \})\\
=& (\{ p_1, p_2, p_6, p_7, p_8 \} \cup \{p_4, p_6, p_7\}) \cap\\
   &(\{ p_6, p_8 \} \cup
   \{p_6\} \cup
   \{ p_7\}) \\
=& \{p_1, p_2, p_4, p_6, p_7, p_8 \} \cap  \{ p_6, p_7, p_8 \} \\
=& \{ p_6, p_7, p_8 \}
\end{align*}

% O^5
\begin{align*}
(\OSem{ (\poss{a} \true \lor \poss{c} \true ) \land \poss{Act} X }{})^5 (\Proc)
=& \OSem{ (\poss{a} \true \lor \poss{c} \true ) \land \poss{Act} X }
   { \{ p_6, p_7, p_8 \}} \\
=& ( \possDenot{a} \Proc \cup \possDenot{c}\Proc) \cap \\
  &(\possDenot{a} \{ p_6, p_7, p_8 \} \cap
  \possDenot{b} \{ p_6, p_7, p_8 \}  \cap
  \possDenot{c}  \{ p_6, p_7, p_8 \})\\
=& (\{ p_1, p_2, p_6, p_7, p_8 \} \cup \{p_4, p_6, p_7\}) \cap\\
   &(\{ p_6, p_8 \} \cup
   \emptyset \cup
   \{ p_7\}) \\
=& \{p_1, p_2, p_4, p_6, p_7, p_8 \} \cap  \{ p_6, p_7, p_8 \} \\
=& \{ p_6, p_7, p_8 \}
\end{align*}

An dieser Stelle haben wir einen Fixpunkt erreicht, da \\
$ \OSem {(\poss {a} \true \lor \poss{c} \true ) \land \necess {Act} X }{ \{ p_6, p_7, p_8 \}}
= \{ p_6, p_7, p_8 \} $.
